ch02-getting-started/CLRS.Ch02.InsertionSort.Impl.fsti
@@ -1,0 +1,32 @@
+(*
+   Insertion Sort - Public interface for the imperative implementation
+*)
+module CLRS.Ch02.InsertionSort.Impl
+
+open Pulse.Lib.Pervasives
+open Pulse.Lib.Array
+open CLRS.Common.SortSpec
+open CLRS.Ch02.InsertionSort.Spec
+
+module A = Pulse.Lib.Array
+module GR = Pulse.Lib.GhostReference
+module SZ = FStar.SizeT
+module Seq = FStar.Seq
+
+val insertion_sort
+  (a: array int)
+  (#s0: Ghost.erased (Seq.seq int))
+  (len: SZ.t)
+  (ctr: GR.ref nat)
+  (#c0: erased nat)
+  : stt unit
+    (A.pts_to a s0 ** GR.pts_to ctr c0 **
+     pure (
+       SZ.v len == Seq.length s0 /\
+       Seq.length s0 <= A.length a /\
+       SZ.v len > 0))
+    (fun _ -> exists* s (cf: nat). A.pts_to a s ** GR.pts_to ctr cf ** pure (
+       Seq.length s == Seq.length s0 /\
+       sorted s /\
+       permutation s0 s /\
+       complexity_bounded cf (reveal c0) (SZ.v len)))
