ch02-getting-started/CLRS.Ch02.InsertionSort.Lemmas.fst
@@ -1,0 +1,31 @@
+(*
+   Insertion Sort - Lemma proofs
+
+   Proves:
+   - lemma_prefix_le_key: prefix elements are <= key
+   - lemma_combine_sorted_regions: combine sorted prefix with key and shifted suffix
+   - lemma_triangle_step: vj*(vj-1)/2 + vj = (vj+1)*vj/2
+*)
+module CLRS.Ch02.InsertionSort.Lemmas
+
+open CLRS.Common.SortSpec
+open Pulse.Lib.BoundedIntegers
+module Seq = FStar.Seq
+
+let lemma_prefix_le_key
+  (s s_outer: Seq.seq int) (vi vj: nat) (key: int)
+  = if vi = 0 then ()
+    else
+      let pred = vi - 1 in
+      assert (pred + 1 == vi);
+      assert (Seq.index s_outer pred <= key);
+      assert (forall (k: nat). k < vi ==> k <= pred);
+      assert (forall (k: nat). k <= pred /\ pred < vj ==> Seq.index s_outer k <= Seq.index s_outer pred);
+      ()
+
+let lemma_combine_sorted_regions
+  (s: Seq.seq int) (vi vj: nat) (key: int)
+  = ()
+
+let lemma_triangle_step (vj: nat)
+  = assert (op_Multiply vj (vj - 1) + op_Multiply 2 vj == op_Multiply vj (vj + 1))
