ch02-getting-started/CLRS.Ch02.InsertionSort.Lemmas.fsti
@@ -1,0 +1,35 @@
+(*
+   Insertion Sort - Lemma signatures
+*)
+module CLRS.Ch02.InsertionSort.Lemmas
+
+open CLRS.Common.SortSpec
+open Pulse.Lib.BoundedIntegers
+module Seq = FStar.Seq
+
+val lemma_prefix_le_key
+  (s s_outer: Seq.seq int) (vi vj: nat) (key: int)
+  : Lemma
+    (requires
+      vi <= vj /\ vj < Seq.length s /\ Seq.length s == Seq.length s_outer /\
+      prefix_sorted s_outer vj /\
+      prefix_sorted s vi /\
+      (forall (k: nat). k < vi ==> Seq.index s k == Seq.index s_outer k) /\
+      (forall (k: nat). k + 1 == vi ==> Seq.index s_outer k <= key))
+    (ensures forall (k: nat). k < vi ==> Seq.index s k <= key)
+
+val lemma_combine_sorted_regions
+  (s: Seq.seq int) (vi vj: nat) (key: int)
+  : Lemma
+    (requires vi <= vj /\ vj < Seq.length s /\
+      prefix_sorted s vi /\
+      Seq.index s vi == key /\
+      (forall (k: nat). k < vi ==> Seq.index s k <= key) /\
+      (forall (k: nat). vi < k /\ k <= vj ==> Seq.index s k > key) /\
+      (forall (k1 k2: nat). vi < k1 /\ k1 <= k2 /\ k2 <= vj ==>
+        Seq.index s k1 <= Seq.index s k2))
+    (ensures prefix_sorted s (vj + 1))
+
+val lemma_triangle_step (vj: nat)
+  : Lemma (requires vj >= 1)
+          (ensures op_Multiply vj (vj - 1) / 2 + vj == op_Multiply (vj + 1) vj / 2)
