ch02-getting-started/CLRS.Ch02.MergeSort.Impl.fsti
@@ -1,0 +1,54 @@
+(*
+   Merge Sort - Public interface for the imperative implementation
+*)
+module CLRS.Ch02.MergeSort.Impl
+
+open Pulse.Lib.Pervasives
+open Pulse.Lib.Array
+open Pulse.Lib.Array.PtsToRange
+open CLRS.Common.SortSpec
+open CLRS.Ch02.MergeSort.Spec
+
+module A = Pulse.Lib.Array
+module GR = Pulse.Lib.GhostReference
+module SZ = FStar.SizeT
+module Seq = FStar.Seq
+
+val merge
+  (a: array int) (lo mid hi: SZ.t)
+  (ctr: GR.ref nat)
+  (#c0: erased nat)
+  (#s1 #s2: Ghost.erased (Seq.seq int))
+  : stt unit
+    (pts_to_range a (SZ.v lo) (SZ.v mid) s1 **
+     pts_to_range a (SZ.v mid) (SZ.v hi) s2 **
+     GR.pts_to ctr c0 **
+     pure (SZ.v lo <= SZ.v mid /\ SZ.v mid <= SZ.v hi /\ sorted s1 /\ sorted s2))
+    (fun _ -> exists* s_out (cf: nat).
+       pts_to_range a (SZ.v lo) (SZ.v hi) s_out **
+       GR.pts_to ctr cf **
+       pure (
+         sorted s_out /\ 
+         permutation (Seq.append s1 s2) s_out /\
+         merge_complexity_bounded cf (reveal c0) (SZ.v lo) (SZ.v hi)))
+
+val merge_sort
+  (a: A.array int)
+  (len: SZ.t)
+  (ctr: GR.ref nat)
+  (#c0: erased nat)
+  (#s0: erased (Seq.seq int))
+  : stt unit
+    (A.pts_to a s0 **
+     GR.pts_to ctr c0 **
+     pure (
+       SZ.v len == Seq.length s0 /\ 
+       SZ.v len == A.length a))
+    (fun _ -> exists* s (cf: nat).
+       A.pts_to a s **
+       GR.pts_to ctr cf **
+       pure (
+         Seq.length s == Seq.length s0 /\
+         sorted s /\
+         permutation s0 s /\
+         sort_complexity_bounded cf (reveal c0) 0 (SZ.v len)))
